src/Compilers/Z/Bounds/Pipeline/ReflectiveTactics.v
@@ -22,6 +22,8 @@ Require Import Crypto.Compilers.Z.Bounds.Interpretation.
 Require Import Crypto.Compilers.Z.Bounds.Relax.
 Require Import Crypto.Compilers.Reify.
 Require Import Crypto.Compilers.Z.Reify.
+Require Import Crypto.Compilers.InterpSideConditions.
+Require Import Crypto.Compilers.Z.InterpSideConditions.
 Require Import Crypto.Compilers.Z.Bounds.Pipeline.Definition.
 Require Import Crypto.Util.Tactics.Head.
 Require Import Crypto.Util.Tactics.SubstLet.
@@ -123,6 +125,45 @@ Ltac unify_abstract_cbv_interp_rhs_reflexivity :=
        unify LHS RHS'; abstract exact_no_check (eq_refl RHS')
   end.
 
+(** *** Boundedness Lemma Side Conditions *)
+(** The tactic [handle_boundedness_side_condition] unfolds relevant
+    identifiers in the side-condition of the boundedness lemma.  It
+    then calls [boundedness_side_condition_solver], which can be
+    overridden. *)
+(** The tactic [boundedness_side_condition_solver] attempts to solve
+    the algebraic side conditions of the boundedness lemma; it leaves
+    them over if it cannot solve them. *)
+Ltac boundedness_side_condition_solver :=
+  repeat match goal with
+         | [ |- _ /\ _ ] => apply conj
+         | [ |- ?x = ?x ] => reflexivity
+         end;
+  try abstract ring.
+Ltac handle_boundedness_side_condition :=
+  (** TODO: This next bit, with repeat intros [? ?], could be done
+        with a single [apply], if we make the right lemma.  We should
+        write that lemma. *)
+  cbv [PointedProp.to_prop Syntax.interp_flat_type Syntax.interp_base_type Syntax.domain Syntax.codomain];
+  repeat match goal with
+         | [ |- forall x : _ * _, _ ]
+           => let a := fresh in let b := fresh in intros [a b]; revert a b
+         | [ |- forall x, _ ]
+           => let x := fresh "x" in intro x
+         end;
+  cbv [id
+         fst snd
+         InterpSideConditions Compilers.InterpSideConditions.InterpSideConditions interp_side_conditions interpf_side_conditions interpf_side_conditions_gen
+         Z.Syntax.Util.interped_op_side_conditions
+         ExprInversion.invert_Abs
+         Syntax.interp_op Syntax.lift_op
+         Syntax.Zinterp_op
+         SmartMap.SmartFlatTypeMapUnInterp SmartMap.SmartValf SmartMap.SmartFlatTypeMapInterp2
+         Syntax.cast_const Syntax.ZToInterp Syntax.interpToZ];
+  cbv [PointedProp.and_pointed_Prop];
+  try match goal with
+      | [ |- True ] => exact I
+      end;
+  boundedness_side_condition_solver.
 
 (** ** Assemble the parts of Pipeline.Definition, in Gallina *)
 (** In this section, we assemble [PreWfPipeline] and [PostWfPipeline],
@@ -144,6 +185,7 @@ Require Import Crypto.Compilers.Z.Syntax.Equality.
 Require Import Crypto.Compilers.Z.Syntax.Util.
 Require Import Crypto.Compilers.Z.Bounds.Interpretation.
 Require Import Crypto.Compilers.Z.Bounds.Relax.
+Require Import Crypto.Util.PointedProp.
 Require Import Crypto.Util.PartiallyReifiedProp.
 Require Import Crypto.Util.Equality.
 
@@ -164,6 +206,7 @@ Section with_round_up_list.
              {fZ}
              {final_e_evar : interp_flat_type Syntax.interp_base_type (pick_type given_output_bounds)}
              {e}
+             {e_pre_pkg}
              {e_pkg}
              (** ** reification *)
              (rexpr_sig : { rexpr : Expr base_type op t | forall x, Interp Syntax.interp_op rexpr x = fZ x })
@@ -174,8 +217,10 @@ Section with_round_up_list.
              (Hwf : forall var1 var2,
                  let P := (@reflect_wfT base_type base_type_eq_semidec_transparent op op_beq var1 var2 nil _ _ (ExprEta' e _) (ExprEta' e _)) in
                  trueify P = P)
+             (** ** post-wf-pre-bounds-pipeline *)
+             (Hpost_wf_pre_bounds : e_pre_pkg = PostWfPreBoundsPipeline opts e)
              (** ** post-wf-pipeline *)
-             (Hpost : e_pkg = PostWfPipeline _ opts e input_bounds)
+             (Hpost : e_pkg = PostWfBoundsPipeline _ opts e e_pre_pkg input_bounds)
              (Hpost_correct : Some {| input_expr := e ; input_bounds := input_bounds ; output_bounds := b ; output_expr := e' |} = e_pkg)
              (** ** renaming *)
              (Hrenaming : e_final = e')
@@ -187,8 +232,9 @@ Section with_round_up_list.
                 = eq_rect _ (fun t => Expr base_type op (Arrow (pick_type input_bounds) t)) e' _ (eq_sym Hbounds_sane))
              (** ** instantiation of original evar *)
              (Hevar : final_e_evar = InterpEta (t:=Arrow _ _) Syntax.interp_op e_final_newtype v')
-             (** ** side condition *)
-             (Hv : Bounds.is_bounded_by input_bounds (cast_back_flat_const v'))
+             (** ** side conditions (boundedness) *)
+             (Hv1 : Bounds.is_bounded_by input_bounds (cast_back_flat_const v'))
+             (Hv2 : forall v, PointedProp.to_prop (InterpSideConditions e_pre_pkg v))
     : Bounds.is_bounded_by given_output_bounds (fZ (cast_back_flat_const v'))
       /\ cast_back_flat_const final_e_evar = fZ (cast_back_flat_const v').
   Proof.
@@ -223,8 +269,8 @@ End with_round_up_list.
 Ltac refine_with_pipeline_correct opts :=
   lazymatch goal with
   | [ |- _ /\ ?castback ?fW = ?fZ ?arg ]
-    => let lem := open_constr:(@PipelineCorrect _ opts _ _ _ _ _ _ _ _ _ _ _ _) in
-       simple refine (lem _ _ _ _ _ _ _ _ _ _ _ _);
+    => let lem := open_constr:(@PipelineCorrect _ opts _ _ _ _ _ _ _ _ _ _ _ _ _) in
+       simple refine (lem _ _ _ _ _ _ _ _ _ _ _ _ _ _);
        subst fW fZ
   end;
   [ eexists
@@ -264,6 +310,8 @@ Ltac solve_side_conditions :=
    unify_abstract_vm_compute_rhs_reflexivity |
    (** ** reflective wf side-condition 2 *)
    unify_abstract_vm_compute_rhs_reflexivity |
+   (** ** post-wf-pre-bounds-pipeline *)
+   unify_abstract_vm_compute_rhs_reflexivity |
    (** ** post-wf pipeline *)
    unify_abstract_vm_compute_rhs_reflexivity |
    (** ** post-wf pipeline gives [Some _] *)
@@ -283,7 +331,9 @@ Ltac solve_side_conditions :=
    (** ** unfolding of [interp] constants *)
    unify_abstract_cbv_interp_rhs_reflexivity |
    (** ** boundedness of inputs *)
-   abstract handle_bounds_from_hyps ].
+   abstract handle_bounds_from_hyps |
+   (** ** boundedness side-condition *)
+   handle_boundedness_side_condition ].
 
 
 (** ** The Entire Pipeline *)
