src/Compilers/Z/MapCastByDeBruijnInterp.v
@@ -4,7 +4,10 @@ Require Import Crypto.Compilers.SmartMap.
 Require Import Crypto.Compilers.Relations.
 Require Import Crypto.Compilers.MapCastByDeBruijnInterp.
 Require Import Crypto.Compilers.Z.Syntax.
+Require Import Crypto.Compilers.Z.Syntax.Util.
 Require Import Crypto.Compilers.Z.MapCastByDeBruijn.
+Require Import Crypto.Compilers.Z.InterpSideConditions.
+Require Import Crypto.Util.PointedProp.
 
 Section language.
   Context {interp_base_type_bounds : base_type -> Type}
@@ -22,12 +25,14 @@ Section language.
   Context (interp_op_bounds_correct
            : forall t tR opc bs
                     (v : interp_flat_type interp_base_type t)
-                    (H : inbounds t bs v),
+                    (H : inbounds t bs v)
+                    (Hside : to_prop (interped_op_side_conditions opc v)),
               inbounds tR (interp_op_bounds t tR opc bs) (interp_op t tR opc v))
           (pull_cast_back
            : forall t tR opc bs
                     (v : interp_flat_type interp_base_type (pick_type bs))
-                    (H : inbounds t bs (cast_back t bs v)),
+                    (H : inbounds t bs (cast_back t bs v))
+                    (Hside : to_prop (interped_op_side_conditions opc (cast_back t bs v))),
               interp_op t tR opc (cast_back t bs v)
               =
               cast_back _ _ (interp_op _ _ (cast_op _ _ opc bs) v)).
@@ -40,7 +45,8 @@ Section language.
         (Hwf : Wf e)
         (input_bounds : interp_flat_type interp_base_type_bounds (domain t))
     : forall {b} e' (He':MapCast e input_bounds = Some (existT _ b e'))
-             v v' (Hv : @inbounds _ input_bounds v /\ cast_back _ _ v' = v),
+             v v' (Hv : @inbounds _ input_bounds v /\ cast_back _ _ v' = v)
+             (Hside : to_prop (InterpSideConditions e v)),
       Interp interp_op_bounds e input_bounds = b
       /\ @inbounds _ b (Interp interp_op e v)
       /\ cast_back _ _ (Interp interp_op e' v') = (Interp interp_op e v).
